spec/abstract/Structures_A.thy
@@ -67,6 +67,8 @@ datatype apiobject_type =
   | EndpointObject
   | NotificationObject
   | CapTableObject
+  | SchedContextObject
+  | ReplyObject
   | ArchObject aobject_type
 
 definition
@@ -112,11 +114,13 @@ datatype cap
            \<comment> \<open>device flag, pointer, size in bits (i.e. @{text "size = 2^bits"}) and freeIndex (i.e. @{text "freeRef = obj_ref + (freeIndex * 2^4)"})\<close>
          | EndpointCap obj_ref badge cap_rights
          | NotificationCap obj_ref badge cap_rights
-         | ReplyCap obj_ref bool
+         | ReplyCap obj_ref
          | CNodeCap obj_ref nat "bool list"
            \<comment> \<open>CNode ptr, number of bits translated, guard\<close>
          | ThreadCap obj_ref
          | DomainCap
+         | SchedContextCap obj_ref
+         | SchedControlCap
          | IRQControlCap
          | IRQHandlerCap irq
          | Zombie obj_ref "nat option" nat
@@ -173,10 +177,7 @@ definition
 
 definition
   is_reply_cap :: "cap \<Rightarrow> bool" where
-  "is_reply_cap cap \<equiv> case cap of ReplyCap _ m \<Rightarrow> \<not> m | _ \<Rightarrow> False"
-definition
-  is_master_reply_cap :: "cap \<Rightarrow> bool" where
-  "is_master_reply_cap cap \<equiv> case cap of ReplyCap _ m \<Rightarrow> m | _ \<Rightarrow> False"
+  "is_reply_cap cap \<equiv> case cap of ReplyCap _ \<Rightarrow> True | _ \<Rightarrow> False"
 definition
   is_zombie :: "cap \<Rightarrow> bool" where
   "is_zombie cap \<equiv> case cap of Zombie _ _ _ \<Rightarrow> True | _ \<Rightarrow> False"
@@ -217,6 +218,11 @@ fun is_ntfn_cap :: "cap \<Rightarrow> bool"
 where
   "is_ntfn_cap (NotificationCap _ _ _) = True"
 | "is_ntfn_cap _                        = False"
+
+fun is_sched_context_cap :: "cap \<Rightarrow> bool"
+where
+  "is_sched_context_cap (SchedContextCap _) = True"
+| "is_sched_context_cap _ = False"
 
 primrec (nonexhaustive)
   cap_rights :: "cap \<Rightarrow> cap_rights"
@@ -317,6 +323,7 @@ datatype ntfn
 record notification =
   ntfn_obj :: ntfn
   ntfn_bound_tcb :: "obj_ref option"
+  ntfn_sc        :: "obj_ref option"
 
 
 definition
@@ -331,7 +338,8 @@ definition
   default_notification :: notification where
   "default_notification \<equiv> \<lparr>
      ntfn_obj = default_ntfn,
-     ntfn_bound_tcb = None \<rparr>"
+     ntfn_bound_tcb = None,
+     ntfn_sc = None \<rparr>"
 
 
 text {* Thread Control Blocks are the in-kernel representation of a thread.
@@ -345,10 +353,7 @@ indicates that the TCB is not currently used by a running thread.
 TCBs also contain some special-purpose capability slots. The CTable slot is a
 capability to a CNode through which the thread accesses capabilities with which
 to perform system calls. The VTable slot is a capability to a virtual address
-space (an architecture-specific capability type) in which the thread runs. If
-the thread has issued a Reply cap to another thread and is awaiting a reply,
-that cap will have a "master" Reply cap as its parent in the Reply slot. The
-Caller slot is used to initially store any Reply cap issued to this thread. The
+space (an architecture-specific capability type) in which the thread runs. The
 IPCFrame slot stores a capability to a memory frame (an architecture-specific
 capability type) through which messages will be sent and received.
 
@@ -368,7 +373,7 @@ datatype thread_state
   = Running
   | Inactive
   | Restart
-  | BlockedOnReceive obj_ref
+  | BlockedOnReceive obj_ref "obj_ref option"
   | BlockedOnSend obj_ref sender_payload
   | BlockedOnReply
   | BlockedOnNotification obj_ref
@@ -379,8 +384,6 @@ type_synonym priority = word8
 record tcb =
  tcb_ctable        :: cap
  tcb_vtable        :: cap
- tcb_reply         :: cap
- tcb_caller        :: cap
  tcb_ipcframe      :: cap
  tcb_state         :: thread_state
  tcb_fault_handler :: cap_ref
@@ -388,8 +391,9 @@ record tcb =
  tcb_fault         :: "fault option"
  tcb_bound_notification     :: "obj_ref option"
  tcb_mcpriority    :: priority
- tcb_arch          :: arch_tcb (* arch_tcb must have a field for user context *)
-
+ tcb_sched_context :: "obj_ref option"
+ tcb_reply         :: "obj_ref option"
+ tcb_arch          :: arch_tcb
 
 text {* Determines whether a thread in a given state may be scheduled. *}
 primrec
@@ -398,20 +402,17 @@ where
   "runnable (Running)               = True"
 | "runnable (Inactive)              = False"
 | "runnable (Restart)               = True"
-| "runnable (BlockedOnReceive x)  = False"
+| "runnable (BlockedOnReceive _ _)  = False"
 | "runnable (BlockedOnSend x y)     = False"
 | "runnable (BlockedOnNotification x) = False"
 | "runnable (IdleThreadState)       = False"
 | "runnable (BlockedOnReply)        = False"
-
 
 definition
   default_tcb :: tcb where
   "default_tcb \<equiv> \<lparr>
       tcb_ctable   = NullCap,
       tcb_vtable   = NullCap,
-      tcb_reply    = NullCap,
-      tcb_caller   = NullCap,
       tcb_ipcframe = NullCap,
       tcb_state    = Inactive,
       tcb_fault_handler = to_bl (0::machine_word),
@@ -419,7 +420,45 @@ definition
       tcb_fault      = None,
       tcb_bound_notification  = None,
       tcb_mcpriority = minBound,
+      tcb_sched_context = None,
+      tcb_reply      = None,
       tcb_arch       = default_arch_tcb\<rparr>"
+
+type_synonym ticks = "64 word"
+type_synonym time  = "64 word"
+
+record refill =
+  r_time   :: time
+  r_amount :: time
+
+record sched_context =
+  sc_period     :: ticks
+  sc_tcb        :: "obj_ref option"
+  sc_ntfn       :: "obj_ref option"
+  sc_refills    :: "refill list"
+  sc_refill_max :: nat
+  sc_replies    :: "obj_ref list"
+
+definition "MIN_REFILLS = 2"
+definition "MAX_REFILLS = 12"
+
+definition
+  default_sched_context :: sched_context where
+  "default_sched_context \<equiv> \<lparr>
+    sc_period     = 0,
+    sc_tcb        = None,
+    sc_ntfn       = None,
+    sc_refills    = [\<lparr>r_time=0, r_amount=0\<rparr>],
+    sc_refill_max = 0,
+    sc_replies    = []
+  \<rparr>"
+
+record reply =
+  reply_caller :: "obj_ref option"
+  reply_sc     :: "obj_ref option"
+
+definition
+  "default_reply = \<lparr> reply_caller = None, reply_sc = None \<rparr>"
 
 text {*
 All kernel objects are CNodes, TCBs, Endpoints, Notifications or architecture
@@ -430,6 +469,8 @@ datatype kernel_object
          | TCB tcb
          | Endpoint endpoint
          | Notification notification
+         | SchedContext sched_context
+         | Reply reply
          | ArchObj (the_arch_obj: arch_kernel_obj)
 
 lemmas kernel_object_cases =
@@ -455,7 +496,9 @@ where
   "obj_bits (CNode sz cs) = cte_level_bits + sz"
 | "obj_bits (TCB t) = tcb_bits"
 | "obj_bits (Endpoint ep) = endpoint_bits"
-| "obj_bits (Notification ntfn) = ntfn_bits"
+| "obj_bits (Notification ntfn) = ntfn_bits" (* RT ARM: 5*)
+| "obj_bits (SchedContext sc) = 8"
+| "obj_bits (Reply r) = 4"
 | "obj_bits (ArchObj ao) = arch_kobj_size ao"
 
 primrec (nonexhaustive)
@@ -467,6 +510,8 @@ where
 | "obj_size (NotificationCap r b R) = 1 << obj_bits (Notification undefined)"
 | "obj_size (CNodeCap r bits g) = 1 << (cte_level_bits + bits)"
 | "obj_size (ThreadCap r) = 1 << obj_bits (TCB undefined)"
+| "obj_size (SchedContextCap r) = 1 << obj_bits (SchedContext undefined)"
+| "obj_size (ReplyCap r) = 1 << obj_bits (Reply undefined)"
 | "obj_size (Zombie r zb n) = (case zb of None \<Rightarrow> 1 << obj_bits (TCB undefined)
                                         | Some n \<Rightarrow> 1 << (cte_level_bits + n))"
 | "obj_size (ArchObjectCap a) = 1 << arch_obj_size a"
@@ -536,6 +581,10 @@ record abstract_state =
   is_original_cap    :: "cslot_ptr \<Rightarrow> bool"
   cur_thread         :: obj_ref
   idle_thread        :: obj_ref
+  consumed_time      :: time     -- "amount of time since kernel time was last updated"
+  cur_time           :: time     -- "current time at kernel entry"
+  cur_sc             :: obj_ref  -- "current scheduling context"
+  reprogram_timer    :: bool     -- "whether we need to reprogram the timer on exit"
   machine_state      :: machine_state
   interrupt_irq_node :: "irq \<Rightarrow> obj_ref"
   interrupt_states   :: "irq \<Rightarrow> irq_state"
@@ -569,7 +618,7 @@ capability slots within a TCB.
 *}
 definition
   tcb_cnode_index :: "nat \<Rightarrow> cnode_index" where
-  "tcb_cnode_index n \<equiv> to_bl (of_nat n :: 3 word)"
+  "tcb_cnode_index n \<equiv> to_bl (of_nat n :: 2 word)"
 
 text {* Zombie capabilities store the bit size of the CNode cap they were
 created from or None if they were created from a TCB cap. This function
@@ -577,11 +626,11 @@ decodes the bit-length of cnode indices into the relevant kernel objects.
 *}
 definition
   zombie_cte_bits :: "nat option \<Rightarrow> nat" where
- "zombie_cte_bits N \<equiv> case N of Some n \<Rightarrow> n | None \<Rightarrow> 3"
+ "zombie_cte_bits N \<equiv> case N of Some n \<Rightarrow> n | None \<Rightarrow> 2"
 
 lemma zombie_cte_bits_simps[simp]:
  "zombie_cte_bits (Some n) = n"
- "zombie_cte_bits None     = 3"
+ "zombie_cte_bits None     = 2"
   by (simp add: zombie_cte_bits_def)+
 
 text {* The first capability slot of the relevant kernel object. *}
@@ -597,7 +646,7 @@ primrec
   obj_refs :: "cap \<Rightarrow> obj_ref set"
 where
   "obj_refs NullCap = {}"
-| "obj_refs (ReplyCap r m) = {}"
+| "obj_refs (ReplyCap r) = {r}"
 | "obj_refs IRQControlCap = {}"
 | "obj_refs (IRQHandlerCap irq) = {}"
 | "obj_refs (UntypedCap dev r s f) = {}"
@@ -606,23 +655,26 @@ where
 | "obj_refs (NotificationCap r b cr) = {r}"
 | "obj_refs (ThreadCap r) = {r}"
 | "obj_refs DomainCap = {}"
+| "obj_refs (SchedContextCap r) = {r}"
+| "obj_refs SchedControlCap = {}"
 | "obj_refs (Zombie ptr b n) = {ptr}"
 | "obj_refs (ArchObjectCap x) = set_option (aobj_ref x)"
 
 text {*
   The partial definition below is sometimes easier to work with.
-  It also provides cases for UntypedCap and ReplyCap which are not
-  true object references in the sense of the other caps.
+  It also provides a result for UntypedCap which does not contain
+  a true object reference in the sense of the other caps.
 *}
 primrec (nonexhaustive)
   obj_ref_of :: "cap \<Rightarrow> obj_ref"
 where
   "obj_ref_of (UntypedCap dev r s f) = r"
-| "obj_ref_of (ReplyCap r m) = r"
+| "obj_ref_of (ReplyCap r) = r"
 | "obj_ref_of (CNodeCap r bits guard) = r"
 | "obj_ref_of (EndpointCap r b cr) = r"
 | "obj_ref_of (NotificationCap r b cr) = r"
 | "obj_ref_of (ThreadCap r) = r"
+| "obj_ref_of (SchedContextCap r) = r"
 | "obj_ref_of (Zombie ptr b n) = ptr"
 | "obj_ref_of (ArchObjectCap x) = the (aobj_ref x)"
 
@@ -636,9 +688,7 @@ definition tcb_cnode_map :: "tcb \<Rightarrow> cnode_index \<Rightarrow> cap opt
   "tcb_cnode_map tcb \<equiv>
    [tcb_cnode_index 0 \<mapsto> tcb_ctable tcb,
     tcb_cnode_index 1 \<mapsto> tcb_vtable tcb,
-    tcb_cnode_index 2 \<mapsto> tcb_reply tcb,
-    tcb_cnode_index 3 \<mapsto> tcb_caller tcb,
-    tcb_cnode_index 4 \<mapsto> tcb_ipcframe tcb]"
+    tcb_cnode_index 2 \<mapsto> tcb_ipcframe tcb]"
 
 definition cap_of :: "kernel_object \<Rightarrow> cnode_index \<Rightarrow> cap option"
   where
