spec/abstract/ARM/Arch_Structs_A.thy
@@ -134,7 +134,7 @@ definition endpoint_bits :: nat where
   "endpoint_bits \<equiv> 4"
 
 definition ntfn_bits :: nat where
-  "ntfn_bits \<equiv> 4"
+  "ntfn_bits \<equiv> 5"
 
 definition untyped_min_bits :: nat where
   "untyped_min_bits \<equiv> 4"
