spec/abstract/ARM/Init_A.thy
@@ -31,6 +31,9 @@ definition
   "init_tcb_ptr = kernel_base + 0x2000"
 
 definition
+  "idle_sc_ptr = kernel_base + 0x3000"
+
+definition
   init_irq_node_ptr :: word32 where
   "init_irq_node_ptr = kernel_base + 0x8000"
 
@@ -69,8 +72,6 @@ definition
   (idle_thread_ptr \<mapsto> TCB \<lparr>
     tcb_ctable = NullCap,
     tcb_vtable = NullCap,
-    tcb_reply = NullCap,
-    tcb_caller = NullCap,
     tcb_ipcframe = NullCap,
     tcb_state = IdleThreadState,
     tcb_fault_handler = replicate word_bits False,
@@ -78,10 +79,13 @@ definition
     tcb_fault = None,
     tcb_bound_notification = None,
     tcb_mcpriority = minBound,
+    tcb_sched_context = Some idle_sc_ptr,
+    tcb_reply = None,
     tcb_arch = init_arch_tcb
   \<rparr>,
-  init_globals_frame \<mapsto> ArchObj (DataPage False ARMSmallPage), (* same reason as why we kept the definition of init_globals_frame *)
-  init_global_pd \<mapsto> ArchObj (PageDirectory global_pd)
+  init_globals_frame \<mapsto> ArchObj (DataPage False ARMSmallPage), (* FIXME: same reason as why we kept the definition of init_globals_frame *)
+  init_global_pd \<mapsto> ArchObj (PageDirectory global_pd),
+  idle_sc_ptr \<mapsto> SchedContext (default_sched_context\<lparr>sc_tcb := Some idle_thread_ptr\<rparr>)
   )"
 
 definition
@@ -99,6 +103,10 @@ definition
     is_original_cap = init_ioc,
     cur_thread = idle_thread_ptr,
     idle_thread = idle_thread_ptr,
+    consumed_time = 0,
+    cur_time = 0,
+    cur_sc = idle_sc_ptr,
+    reprogram_timer = False,
     machine_state = init_machine_state,
     interrupt_irq_node = \<lambda>irq. init_irq_node_ptr + (ucast irq << cte_level_bits),
     interrupt_states = \<lambda>_. Structures_A.IRQInactive,
