spec/abstract/Retype_A.thy
@@ -43,8 +43,9 @@ where
 | "default_cap Untyped oref s dev = UntypedCap dev oref s 0"
 | "default_cap TCBObject oref s _ = ThreadCap oref"
 | "default_cap EndpointObject oref s _ = EndpointCap oref 0 UNIV"
-| "default_cap NotificationObject oref s _ =
-     NotificationCap oref 0 {AllowRead, AllowWrite}"
+| "default_cap NotificationObject oref s _ = NotificationCap oref 0 {AllowRead, AllowWrite}"
+| "default_cap SchedContextObject oref s _ = SchedContextCap oref"
+| "default_cap ReplyObject oref _ _ = ReplyCap oref"
 | "default_cap (ArchObject aobj) oref s dev = ArchObjectCap (arch_default_cap aobj oref s dev)"
 
 text {* Create and install a new capability to a newly created object. *}
@@ -78,6 +79,8 @@ definition
          | TCBObject \<Rightarrow> TCB default_tcb
          | EndpointObject \<Rightarrow> Endpoint default_ep
          | NotificationObject \<Rightarrow> Notification default_notification
+         | SchedContextObject \<Rightarrow> SchedContext default_sched_context
+         | ReplyObject \<Rightarrow> Reply default_reply
          | ArchObject aobj \<Rightarrow> ArchObj (default_arch_object aobj dev n)"
 
 text {* The size in bits of the objects that will be created when a given type
@@ -90,6 +93,8 @@ definition
          | TCBObject \<Rightarrow> obj_bits (TCB default_tcb)
          | EndpointObject \<Rightarrow> obj_bits (Endpoint undefined)
          | NotificationObject \<Rightarrow> obj_bits (Notification undefined)
+         | SchedContextObject \<Rightarrow> obj_bits (SchedContext undefined)
+         | ReplyObject \<Rightarrow> obj_bits (Reply default_reply)
          | ArchObject aobj \<Rightarrow> obj_bits $ ArchObj $ default_arch_object aobj False obj_size_bits"
 
 section "Main Retype Implementation"
