spec/abstract/SchedContext_A.thy
@@ -1,0 +1,445 @@
+(*
+ * Copyright 2016, Data61, CSIRO
+ *
+ * This software may be distributed and modified according to the terms of
+ * the GNU General Public License version 2. Note that NO WARRANTY is provided.
+ * See "LICENSE_GPLv2.txt" for details.
+ *
+ * @TAG(DATA61_GPL)
+ *)
+
+chapter "Scheduling Contexts and Control"
+
+theory SchedContext_A
+imports IpcCancel_A Invocations_A
+begin
+
+text \<open> This theory contains operations on scheduling contexts and scheduling control. \<close>
+
+definition "MIN_BUDGET = 2 * kernelWCET_ticks"
+definition "MIN_BUDGET_US = 2 * kernelWCET_us"
+
+
+definition
+  get_tcb_sc :: "obj_ref \<Rightarrow> (sched_context,'z::state_ext) s_monad"
+where
+  "get_tcb_sc tcb_ptr = do
+    sc_opt \<leftarrow> thread_get tcb_sched_context tcb_ptr;
+    sc_ptr \<leftarrow> assert_opt sc_opt;
+    get_sched_context sc_ptr
+  od"
+
+abbreviation
+  "refill_hd sc \<equiv> hd (sc_refills sc)"
+
+definition
+  get_sc_time :: "obj_ref \<Rightarrow> time det_ext_monad"
+where
+  "get_sc_time tcb_ptr = do
+    sc \<leftarrow> get_tcb_sc tcb_ptr;
+    return $ r_time (refill_hd sc)
+  od"
+
+
+text \<open>Enqueue a TCB in the release queue, sorted by release time of
+  the corresponding scheduling context.\<close>
+definition
+  tcb_release_enqueue :: "obj_ref \<Rightarrow> unit det_ext_monad"
+where
+  "tcb_release_enqueue tcb_ptr = do
+     time \<leftarrow> get_sc_time tcb_ptr;
+     qs \<leftarrow> gets release_queue;
+     times \<leftarrow> mapM get_sc_time qs;
+     qst \<leftarrow> return $ zip qs times;
+     qst' \<leftarrow> return $ filter (\<lambda>(_,t'). t' \<le> time) qst @ [(tcb_ptr,time)] @ filter (\<lambda>(_,t'). \<not>t' \<le> time) qst;
+     modify (\<lambda>s. s\<lparr>release_queue := map fst qst'\<rparr>)
+  od"
+
+definition
+  refills_capacity :: "time \<Rightarrow> refill list \<Rightarrow> time"
+where
+  "refills_capacity usage refills \<equiv>
+  if r_amount (hd refills) < usage then 0 else r_amount (hd refills) - usage"
+
+definition
+  get_refills :: "obj_ref \<Rightarrow> (refill list, 'z::state_ext) s_monad"
+where
+  "get_refills sc_ptr = do
+    sc \<leftarrow> get_sched_context sc_ptr;
+    return $ sc_refills sc
+  od"
+
+definition
+  refill_capacity :: "obj_ref \<Rightarrow> time \<Rightarrow> (time, 'z::state_ext) s_monad"
+where
+  "refill_capacity sc_ptr usage = do
+    refills \<leftarrow> get_refills sc_ptr;
+    return $ refills_capacity usage refills
+  od"
+
+definition
+  sufficient_refills :: "time \<Rightarrow> refill list \<Rightarrow> bool"
+where
+  "sufficient_refills usage refills = (MIN_BUDGET < refills_capacity usage refills)"
+
+definition
+  refill_sufficient :: "obj_ref \<Rightarrow> time \<Rightarrow> (bool, 'z::state_ext) s_monad"
+where
+  "refill_sufficient sc_ptr usage = do
+    refills \<leftarrow> get_refills sc_ptr;
+    return $ sufficient_refills usage refills
+  od"
+
+definition
+  refill_ready :: "obj_ref \<Rightarrow> (bool, 'z::state_ext) s_monad"
+where
+  "refill_ready sc_ptr = do
+    cur_time \<leftarrow> gets cur_time;
+    sc \<leftarrow> get_sched_context sc_ptr;
+    sc_time \<leftarrow> return $ r_time (refill_hd sc);
+    return $ sc_time \<le> cur_time + kernelWCET_ticks
+  od"
+
+definition
+  refill_size :: "obj_ref \<Rightarrow> (nat, 'z::state_ext) s_monad"
+where
+  "refill_size sc_ptr = do
+    refills \<leftarrow> get_refills sc_ptr;
+    return $ size refills
+  od"
+
+definition
+  refill_single :: "obj_ref \<Rightarrow> (bool, 'z::state_ext) s_monad"
+where
+  "refill_single sc_ptr = do
+    sz \<leftarrow> refill_size sc_ptr;
+    return (sz = 1)
+  od"
+
+definition
+  refills_sum :: "refill list \<Rightarrow> time"
+where
+  "refills_sum rf = \<Sum> (set (map r_amount rf))"
+
+definition
+  refill_sum :: "obj_ref \<Rightarrow> (time, 'z::state_ext) s_monad"
+where
+  "refill_sum sc_ptr = do
+    refills \<leftarrow> get_refills sc_ptr;
+    return $ refills_sum refills
+  od"
+
+definition
+  set_refills :: "obj_ref \<Rightarrow> refill list \<Rightarrow> (unit, 'z::state_ext) s_monad"
+where
+  "set_refills sc_ptr refills = do
+    sc \<leftarrow> get_sched_context sc_ptr;
+    set_sched_context sc_ptr (sc\<lparr>sc_refills:= refills\<rparr>)
+  od"
+
+definition
+  refill_pop_head :: "obj_ref \<Rightarrow> (refill, 'z::state_ext) s_monad"
+where
+  "refill_pop_head sc_ptr = do
+    refills \<leftarrow> get_refills sc_ptr;
+    assert (1 < size refills);
+    set_refills sc_ptr (tl refills);
+    return $ hd refills
+  od"
+
+definition
+  refill_add_tail :: "obj_ref \<Rightarrow> refill \<Rightarrow> (unit, 'z::state_ext) s_monad"
+where
+  "refill_add_tail sc_ptr rfl = do
+    assert (r_amount rfl \<noteq> 0);
+    sc \<leftarrow> get_sched_context sc_ptr;
+    refills \<leftarrow> return $ sc_refills sc;
+    assert (size refills < sc_refill_max sc);
+    set_refills sc_ptr (refills @ [rfl])
+  od"
+
+definition
+  refill_new :: "obj_ref \<Rightarrow> nat \<Rightarrow> ticks \<Rightarrow> ticks \<Rightarrow> (unit, 'z::state_ext) s_monad"
+where
+  "refill_new sc_ptr max_refills budget period = do
+    sc \<leftarrow> get_sched_context sc_ptr;
+    assert (MIN_BUDGET < budget);
+    cur_time \<leftarrow> gets cur_time;
+    refill \<leftarrow> return \<lparr> r_time = cur_time, r_amount = budget \<rparr>;
+    sc' \<leftarrow> return $ sc\<lparr> sc_period := period, sc_refills := [refill], sc_refill_max := max_refills \<rparr>;
+    set_sched_context sc_ptr sc'
+  od"
+
+
+definition
+  merge_refill :: "refill \<Rightarrow> refill \<Rightarrow> refill"
+where
+  "merge_refill r1 r2 = \<lparr> r_time = r_time r1, r_amount = r_amount r2 + r_amount r1 \<rparr>"
+
+definition
+  "can_merge_refill r1 r2 \<equiv> r_time r2 \<le> r_time r1 + r_amount r1"
+
+fun
+  refills_merge_prefix :: "refill list \<Rightarrow> refill list"
+where
+  "refills_merge_prefix [] = []"
+| "refills_merge_prefix [r] = [r]"
+| "refills_merge_prefix (r1 # r2 # rs) = 
+     (if can_merge_refill r1 r2
+      then refills_merge_prefix (merge_refill r1 r2 # rs)
+      else r1 # r2 # rs)"
+
+definition
+  refill_unblock_check :: "obj_ref \<Rightarrow> (unit, 'z::state_ext) s_monad"
+where
+  "refill_unblock_check sc_ptr = do
+    ct \<leftarrow> gets cur_time;
+    refills \<leftarrow> get_refills sc_ptr;
+    refills' \<leftarrow> return $ refills_merge_prefix ((hd refills)\<lparr>r_time := ct\<rparr> # tl refills);
+    refills'' \<leftarrow> return (if sufficient_refills 0 refills' then refills' else
+      let
+        r1 = hd refills';
+        r2 = hd (tl refills');
+        rs = tl (tl refills')
+      in \<lparr> r_time = r_time r2, r_amount = r_amount r2 + r_amount r1 \<rparr> # rs);
+    set_refills sc_ptr refills''
+  od"
+
+function
+  refills_budget_check :: "ticks \<Rightarrow> ticks \<Rightarrow> refill list \<Rightarrow> ticks \<times> refill list"
+where
+  "refills_budget_check period usage [] = (usage, [])"
+| "refills_budget_check period usage (r#rs) = (if r_amount r \<le> usage \<and> 0 < r_amount r
+     then refills_budget_check period (usage - r_amount r) (rs @ [r\<lparr>r_time := r_time r + period\<rparr>]) 
+     else (usage, r#rs))"
+  by pat_completeness auto
+
+termination refills_budget_check
+  apply (relation "measure (\<lambda>(p,u,rs). unat u)")
+   apply clarsimp
+  apply unat_arith
+  done
+
+definition
+  refill_budget_check :: "obj_ref \<Rightarrow> ticks \<Rightarrow> (ticks, 'z::state_ext) s_monad"
+where
+  "refill_budget_check sc_ptr usage = do    
+    sc \<leftarrow> get_sched_context sc_ptr;
+    period \<leftarrow> return $ sc_period sc;
+    refills \<leftarrow> return $ sc_refills sc;
+    rfhd \<leftarrow> return $ hd refills;
+
+    (usage', refills') \<leftarrow> return $ refills_budget_check period usage refills;
+
+    refills'' \<leftarrow> return (if 0 < usage' \<and> 0 < period then
+      let r1 = hd refills'; 
+          r1' = r1 \<lparr>r_time := r_time r1 + usage\<rparr>;
+          rs = tl refills'
+      in if rs \<noteq> [] \<and> can_merge_refill r1' (hd rs) then merge_refill r1' (hd rs) # tl rs else [r1]
+    else refills');
+
+    set_refills sc_ptr refills';
+
+    return usage'
+  od"
+
+definition
+  refill_split_check :: "obj_ref \<Rightarrow> time \<Rightarrow> (unit, 'z::state_ext) s_monad"
+where
+  "refill_split_check sc_ptr usage = do
+    ct \<leftarrow> gets cur_time;
+    sc \<leftarrow> get_sched_context sc_ptr;
+    refills \<leftarrow> return $ sc_refills sc;
+    rfhd \<leftarrow> return $ hd refills;
+    assert (0 < usage \<and> usage \<le> r_amount rfhd);
+    assert (r_time rfhd \<le> ct);
+
+    remaining \<leftarrow> return $ r_amount rfhd - usage;
+    if remaining < MIN_BUDGET \<and> size refills = 1
+    then
+      set_refills sc_ptr [\<lparr> r_time = r_time rfhd + sc_period sc, r_amount = r_amount rfhd \<rparr>]
+    else do
+      if size refills = sc_refill_max sc \<or> remaining < MIN_BUDGET
+      then
+        let r2 = hd (tl refills); rs = tl (tl refills) in
+        set_refills sc_ptr (r2 \<lparr>r_amount := r_amount r2 + remaining\<rparr> # rs)
+      else
+        set_refills sc_ptr (rfhd\<lparr>r_amount := remaining\<rparr> # tl refills);
+      new \<leftarrow> return \<lparr> r_time = r_time rfhd + sc_period sc, r_amount = usage \<rparr>;
+      refill_add_tail sc_ptr new
+    od
+  od"
+
+
+definition
+  refill_update :: "obj_ref \<Rightarrow> ticks \<Rightarrow> ticks \<Rightarrow> nat \<Rightarrow> (unit, 'z::state_ext) s_monad"
+where
+  "refill_update sc_ptr new_period new_budget new_max_refills =
+    refill_new sc_ptr new_max_refills new_budget new_period
+    (* RT: may need to tweak this in the future *)
+  "
+
+definition
+  postpone :: "obj_ref \<Rightarrow> (unit, 'z::state_ext) s_monad"
+where
+  "postpone sc_ptr = do
+    sc \<leftarrow> get_sched_context sc_ptr;
+    tcb_ptr \<leftarrow> assert_opt $ sc_tcb sc;
+    do_extended_op $ tcb_sched_action tcb_sched_dequeue tcb_ptr;
+    do_extended_op $ tcb_release_enqueue tcb_ptr;
+    modify (\<lambda>s. s\<lparr> reprogram_timer := True \<rparr>)
+  od"
+
+text \<open>
+  Resume a scheduling context: check if the bound TCB
+  is runnable and add it to the scheduling queue if required
+\<close> 
+definition
+  sched_context_resume :: "obj_ref \<Rightarrow> (unit, 'z::state_ext) s_monad"
+where
+  "sched_context_resume sc_ptr \<equiv> do
+     sc \<leftarrow> get_sched_context sc_ptr;
+     tptr \<leftarrow> assert_opt $ sc_tcb sc;
+     in_release_q \<leftarrow> select_ext (in_release_queue tptr) {True,False};
+     sched \<leftarrow> is_schedulable tptr in_release_q;
+     when sched $ do
+       refill_unblock_check sc_ptr;
+       ts \<leftarrow> thread_get tcb_state tptr;
+       ready \<leftarrow> refill_ready sc_ptr;
+       sufficient \<leftarrow> refill_sufficient sc_ptr 0;
+       when (runnable ts \<and> 0 < sc_refill_max sc \<and> \<not>(ready \<and> sufficient)) $ postpone sc_ptr
+     od
+   od"
+
+
+text \<open>  Bind a TCB to a scheduling context. \<close>
+definition
+  sched_context_bind_tcb :: "obj_ref \<Rightarrow> obj_ref \<Rightarrow> unit det_ext_monad"
+where
+  "sched_context_bind_tcb sc_ptr tcb_ptr = do
+    sc \<leftarrow> get_sched_context sc_ptr;
+    set_sched_context sc_ptr (sc\<lparr>sc_tcb := Some tcb_ptr\<rparr>);
+    thread_set (\<lambda>tcb. tcb\<lparr>tcb_sched_context := Some sc_ptr\<rparr>) tcb_ptr; 
+    sched_context_resume sc_ptr;
+    inq \<leftarrow> gets $ in_release_queue tcb_ptr;
+    sched \<leftarrow> is_schedulable tcb_ptr inq;
+    when sched $ switch_if_required_to tcb_ptr
+  od"
+
+text \<open> Unbind TCB from its scheduling context, if there is one bound. \<close>
+definition
+  unbind_from_sc :: "obj_ref \<Rightarrow> (unit, 'z::state_ext) s_monad"
+where
+  "unbind_from_sc tcb_ptr = do
+    sc_ptr_opt \<leftarrow> thread_get tcb_sched_context tcb_ptr;
+    maybeM sched_context_unbind_tcb sc_ptr_opt
+  od"
+
+definition
+  maybe_donate_sc :: "obj_ref \<Rightarrow> obj_ref \<Rightarrow> unit det_ext_monad"
+where
+  "maybe_donate_sc tcb_ptr ntfn_ptr = do
+     sc_opt \<leftarrow> thread_get tcb_sched_context tcb_ptr;
+     when (sc_opt = None) $ 
+       liftM ntfn_sc (get_notification ntfn_ptr) >>= maybeM (\<lambda>sc_ptr. do
+         sc_tcb \<leftarrow> liftM sc_tcb $ get_sched_context sc_ptr;
+         when (sc_tcb = None) $ sched_context_donate sc_ptr tcb_ptr
+       od)
+   od"
+
+definition
+  maybe_return_sc :: "obj_ref \<Rightarrow> obj_ref \<Rightarrow> unit det_ext_monad"
+where
+  "maybe_return_sc ntfn_ptr tcb_ptr = do
+    nsc_opt \<leftarrow> liftM ntfn_sc $ get_notification ntfn_ptr;
+    tsc_opt \<leftarrow> thread_get tcb_sched_context tcb_ptr;
+    when (nsc_opt = tsc_opt \<and> nsc_opt \<noteq> None) $ do
+      sc_ptr \<leftarrow> assert_opt nsc_opt;
+      thread_set (tcb_sched_context_update $ K None) tcb_ptr;
+      sc \<leftarrow> get_sched_context sc_ptr;
+      set_sched_context sc_ptr (sc\<lparr>sc_tcb:= None\<rparr>)
+    od
+  od"
+
+text \<open> User-level scheduling context invocations. \<close>
+definition
+  invoke_sched_context :: "sched_context_invocation \<Rightarrow> (unit, det_ext) se_monad"
+where
+  "invoke_sched_context iv \<equiv> liftE $ case iv of
+    InvokeSchedContextBind sc_ptr cap \<Rightarrow> (case cap of
+      ThreadCap tcb_ptr \<Rightarrow> sched_context_bind_tcb sc_ptr tcb_ptr
+    | NotificationCap ntfn _ _ \<Rightarrow> sched_context_bind_ntfn sc_ptr ntfn
+    | _ \<Rightarrow> fail)
+  | InvokeSchedContextUnbindObject sc_ptr cap \<Rightarrow> (case cap of
+      ThreadCap _ \<Rightarrow> sched_context_unbind_tcb sc_ptr
+    | NotificationCap _ _ _ \<Rightarrow> sched_context_unbind_ntfn sc_ptr
+    | _ \<Rightarrow> fail)
+  | InvokeSchedContextUnbind sc_ptr \<Rightarrow> do
+      sched_context_unbind_all_tcbs sc_ptr;
+      sched_context_unbind_ntfn sc_ptr
+    od"
+
+text \<open> The Scheduling Control invocation configures the budget of a scheduling context. \<close>
+definition
+  invoke_sched_control_configure :: "sched_control_invocation \<Rightarrow> (unit, det_ext) se_monad"
+where
+  "invoke_sched_control_configure iv \<equiv>
+  case iv of InvokeSchedControlConfigure sc_ptr budget period mrefills \<Rightarrow> liftE $ do
+    sc \<leftarrow> get_sched_context sc_ptr;
+    period \<leftarrow> return (if budget = period then 0 else period);
+    when (sc_tcb sc \<noteq> None) $ do
+      tcb_ptr \<leftarrow> assert_opt $ sc_tcb sc;
+      do_extended_op $ tcb_release_remove tcb_ptr;
+      st \<leftarrow> get_thread_state tcb_ptr;
+      if 0 < sc_refill_max sc \<and> runnable st then do
+        refill_update sc_ptr period budget mrefills;
+        sched_context_resume sc_ptr;
+        switch_if_required_to tcb_ptr
+      od
+      else
+        refill_new sc_ptr mrefills budget period
+    od
+  od"
+
+
+text \<open> Update time consumption of current scheduling context and current domain. \<close>
+definition
+  commit_time :: "(unit, 'z::state_ext) s_monad"
+where
+  "commit_time = do
+    consumed \<leftarrow> gets consumed_time;
+    ct \<leftarrow> gets cur_thread;
+    it \<leftarrow> gets idle_thread;
+    when (0 < consumed \<and> ct \<noteq> it) $ do
+      csc \<leftarrow> gets cur_sc;
+      refill_split_check csc consumed
+    od;
+    do_extended_op $ commit_domain_time;
+    modify (\<lambda>s. s\<lparr>consumed_time := 0\<rparr> )
+  od"
+
+
+section "Global time"
+
+definition
+  rollback_time :: "(unit, 'z::state_ext) s_monad"
+where
+  "rollback_time = do
+    consumed \<leftarrow> gets consumed_time;
+    modify (\<lambda>s. s\<lparr>cur_time := cur_time s - consumed \<rparr>);
+    modify (\<lambda>s. s\<lparr>consumed_time := 0\<rparr> )
+  od"
+
+
+text \<open>Update current and consumed time.\<close>
+definition
+  update_time_stamp :: "(unit, 'z::state_ext) s_monad"
+where
+  "update_time_stamp = do
+    prev_time \<leftarrow> gets cur_time;
+    cur_time' \<leftarrow> do_machine_op getCurrentTime;
+    modify (\<lambda>s. s\<lparr> cur_time := cur_time' \<rparr>);
+    modify (\<lambda>s. s\<lparr> consumed_time := cur_time' - prev_time \<rparr>)
+  od"
+
+end
