spec/abstract/Syscall_A.thy
@@ -158,72 +158,91 @@ preemptable.
 *}
 
 fun
-  perform_invocation :: "bool \<Rightarrow> bool \<Rightarrow> invocation \<Rightarrow> (data list,'z::state_ext) p_monad"
+  perform_invocation :: "bool \<Rightarrow> bool \<Rightarrow> bool \<Rightarrow> invocation \<Rightarrow> (data list, det_ext) p_monad"
 where
-  "perform_invocation block call (InvokeUntyped i) =
+  "perform_invocation _ _ _ (InvokeUntyped i) =
     doE
       invoke_untyped i;
       returnOk []
     odE"
 
-| "perform_invocation block call (InvokeEndpoint ep badge canGrant) =
+| "perform_invocation block call can_donate (InvokeEndpoint ep badge can_grant) =
     (without_preemption $ do
        thread \<leftarrow> gets cur_thread;
-       send_ipc block call badge canGrant thread ep;
+       send_ipc block call badge can_grant can_donate thread ep;
        return []
      od)"
 
-| "perform_invocation block call (InvokeNotification ep badge) =
+| "perform_invocation _ _ _ (InvokeNotification ep badge) =
     doE
       without_preemption $ send_signal ep badge;
       returnOk []
     odE"
 
-| "perform_invocation block call (InvokeTCB i) = invoke_tcb i"
+| "perform_invocation _ _ _ (InvokeTCB i) = invoke_tcb i"
 
-| "perform_invocation block call (InvokeDomain tptr d) = invoke_domain tptr d"
+| "perform_invocation _ _ _ (InvokeDomain tptr d) = invoke_domain tptr d"
 
-| "perform_invocation block call (InvokeReply thread slot) =
+| "perform_invocation _ _ _ (InvokeReply reply) =
     liftE (do
       sender \<leftarrow> gets cur_thread;
-      do_reply_transfer sender thread slot;
+      do_reply_transfer sender reply;
       return []
     od)"
 
-| "perform_invocation block call (InvokeCNode i) =
+| "perform_invocation _ _ _ (InvokeCNode i) =
     doE
       invoke_cnode i;
       returnOk []
     odE"
 
-| "perform_invocation block call (InvokeIRQControl i) =
+| "perform_invocation _ _ _ (InvokeIRQControl i) =
    doE
      invoke_irq_control i;
      returnOk []
    odE"
 
-| "perform_invocation block call (InvokeIRQHandler i) =
+| "perform_invocation _ _ _ (InvokeIRQHandler i) =
    doE
      liftE $ invoke_irq_handler i;
      returnOk []
    odE"
 
-| "perform_invocation block call (InvokeArchObject i) =
+| "perform_invocation _ _ _ (InvokeSchedContext i) =
+   doE
+     liftE $ invoke_sched_context i;
+     returnOk []
+   odE"
+
+| "perform_invocation _ _ _ (InvokeSchedControl i) =
+   doE
+     liftE $ invoke_sched_control_configure i;
+     returnOk []
+   odE"
+
+| "perform_invocation _ _ _ (InvokeArchObject i) =
     arch_perform_invocation i"
 
+definition
+  get_cap_reg :: "register \<Rightarrow> cap_ref det_ext_monad"
+where
+  "get_cap_reg reg = do
+    ct \<leftarrow> gets cur_thread;
+    liftM data_to_cptr $ as_user ct $ get_register reg
+  od"
 
 definition
-  handle_invocation :: "bool \<Rightarrow> bool \<Rightarrow> (unit,'z::state_ext) p_monad"
+  handle_invocation :: "bool \<Rightarrow> bool \<Rightarrow> bool \<Rightarrow> cap_ref \<Rightarrow> (unit, det_ext) p_monad"
 where
-  "handle_invocation calling blocking \<equiv> doE
+  "handle_invocation calling blocking can_donate cptr \<equiv> doE
     thread \<leftarrow> liftE $ gets cur_thread;
     info \<leftarrow> without_preemption $ get_message_info thread;
     ptr \<leftarrow> without_preemption $ liftM data_to_cptr $
           as_user thread $ getRegister cap_register;
     syscall
       (doE
-         (cap, slot) \<leftarrow> cap_fault_on_failure (of_bl ptr) False $
-                           lookup_cap_and_slot thread ptr;
+         (cap, slot) \<leftarrow> cap_fault_on_failure (of_bl cptr) False $
+                           lookup_cap_and_slot thread cptr;
          buffer \<leftarrow> liftE $ lookup_ipc_buffer False thread;
          extracaps \<leftarrow> lookup_extra_caps thread buffer info;
          returnOk (slot, cap, extracaps, buffer)
@@ -231,13 +250,13 @@ where
       (\<lambda>fault. when blocking $ handle_fault thread fault)
       (\<lambda>(slot,cap,extracaps,buffer). doE
             args \<leftarrow> liftE $ get_mrs thread buffer info;
-            decode_invocation (mi_label info) args ptr slot cap extracaps
+            decode_invocation (mi_label info) args cptr slot cap extracaps
        odE)
       (\<lambda>err. when calling $
             reply_from_kernel thread $ msg_from_syscall_error err)
       (\<lambda>oper. doE
             without_preemption $ set_thread_state thread Restart;
-            reply \<leftarrow> perform_invocation blocking calling oper;
+            reply \<leftarrow> perform_invocation blocking calling can_donate oper;
             without_preemption $ do
                 state \<leftarrow> get_thread_state thread;
                 case state of
@@ -253,48 +272,62 @@ where
 
 
 definition
-  handle_yield :: "(unit,'z::state_ext) s_monad" where
+  handle_yield :: "unit det_ext_monad" where
   "handle_yield \<equiv> do
-     thread \<leftarrow> gets cur_thread;
-     do_extended_op (tcb_sched_action (tcb_sched_dequeue) thread);
-     do_extended_op (tcb_sched_action (tcb_sched_append) thread);
-     do_extended_op (reschedule_required)
+     cur_sc \<leftarrow> gets cur_sc;
+     consumed \<leftarrow> gets consumed_time;
+     refill_budget_check cur_sc consumed;
+     modify $ consumed_time_update $ K 0;
+     end_timeslice;
+     reschedule_required
    od"
 
 definition
-  handle_send :: "bool \<Rightarrow> (unit,'z::state_ext) p_monad" where
-  "handle_send bl \<equiv> handle_invocation False bl"
+  handle_send :: "bool \<Rightarrow> (unit, det_ext) p_monad" where
+  "handle_send bl \<equiv> do
+    cptr \<leftarrow> get_cap_reg cap_register;
+    handle_invocation False bl False cptr
+  od"
 
 definition
-  handle_call :: "(unit,'z::state_ext) p_monad" where
- "handle_call \<equiv> handle_invocation True True"
+  handle_call :: "(unit, det_ext) p_monad" where
+ "handle_call \<equiv>  do
+    cptr \<leftarrow> get_cap_reg cap_register;
+    handle_invocation True True True cptr
+  od"
 
 definition
-  delete_caller_cap :: "obj_ref \<Rightarrow> (unit,'z::state_ext) s_monad" where
- "delete_caller_cap t \<equiv> cap_delete_one (t, tcb_cnode_index 3)"
+  lookup_reply :: "(cap, det_ext) f_monad"
+where
+  "lookup_reply = doE
+    cref \<leftarrow> liftE $ get_cap_reg replyRegister;
+    ct \<leftarrow> liftE $ gets cur_thread;
+    cap \<leftarrow> cap_fault_on_failure (of_bl cref) True $ lookup_cap ct cref;
+    if is_reply_cap cap
+    then returnOk cap
+    else throwError $ CapFault (of_bl cref) True (MissingCapability 0)
+  odE"
 
 definition
-  handle_recv :: "bool \<Rightarrow> (unit,'z::state_ext) s_monad" where
-  "handle_recv is_blocking \<equiv> do
+  handle_recv :: "bool \<Rightarrow> bool \<Rightarrow> (unit, det_ext) s_monad" where
+  "handle_recv is_blocking can_reply \<equiv> do
      thread \<leftarrow> gets cur_thread;
 
      ep_cptr \<leftarrow> liftM data_to_cptr $ as_user thread $
                  getRegister cap_register;
 
-     (cap_fault_on_failure (of_bl ep_cptr) True $ doE
-        ep_cap \<leftarrow> lookup_cap thread ep_cptr;
+     doE
+        ep_cap \<leftarrow> cap_fault_on_failure (of_bl ep_cptr) True (lookup_cap thread ep_cptr);
 
-        let flt = (throwError $ MissingCapability 0)
+        let flt = throwError $ CapFault (of_bl ep_cptr) True (MissingCapability 0)
         in
         case ep_cap
-          of EndpointCap ref badge rights \<Rightarrow>
-             (if AllowRecv \<in> rights
-              then liftE $ do
-                 delete_caller_cap thread;
-                 receive_ipc thread ep_cap is_blocking
-                od
-              else flt)
-           | NotificationCap ref badge rights \<Rightarrow>
+          of EndpointCap ref badge rights \<Rightarrow> doE
+               whenE (AllowRecv \<notin> rights) flt;
+               reply_cap \<leftarrow> if can_reply then lookup_reply else returnOk NullCap;
+               liftE $ receive_ipc thread ep_cap is_blocking reply_cap
+             odE
+           | NotificationCap ref badge rights \<Rightarrow> 
              (if AllowRecv \<in> rights
               then doE
                 ntfn \<leftarrow> liftE $ get_notification ref;
@@ -305,51 +338,61 @@ definition
                odE
               else flt)
            | _ \<Rightarrow> flt
-      odE)
+      odE
       <catch> handle_fault thread
    od"
-
-definition
-  handle_reply :: "(unit,'z::state_ext) s_monad" where
- "handle_reply \<equiv> do
-    thread \<leftarrow> gets cur_thread;
-    caller_cap \<leftarrow> get_cap (thread, tcb_cnode_index 3);
-    case caller_cap of
-      ReplyCap caller False \<Rightarrow> do_reply_transfer thread caller (thread, tcb_cnode_index 3)
-    | NullCap \<Rightarrow> return ()
-    | _ \<Rightarrow> fail
-  od"
 
 
 section {* Top-level event handling  *}
 
 fun
-  handle_event :: "event \<Rightarrow> (unit,'z::state_ext) p_monad"
+  handle_event :: "event \<Rightarrow> (unit, det_ext) p_monad"
 where
-  "handle_event (SyscallEvent call) =
-   (case call of
+  "handle_event (SyscallEvent call) = doE
+    liftE $ update_time_stamp;
+    restart \<leftarrow> liftE $ check_budget_restart;
+    whenE restart (case call of
           SysSend \<Rightarrow> handle_send True
         | SysNBSend \<Rightarrow> handle_send False
         | SysCall \<Rightarrow> handle_call
-        | SysRecv \<Rightarrow> without_preemption $ handle_recv True
+        | SysRecv \<Rightarrow> without_preemption $ handle_recv True True
         | SysYield \<Rightarrow> without_preemption handle_yield
-        | SysReply \<Rightarrow> without_preemption handle_reply
         | SysReplyRecv \<Rightarrow> without_preemption $ do
-            handle_reply;
-            handle_recv True
+            reply_cptr \<leftarrow> get_cap_reg replyRegister;
+            handle_invocation False False True reply_cptr;
+            handle_recv True True
           od
-        | SysNBRecv \<Rightarrow> without_preemption $ handle_recv False)"
+        | SysNBSendRecv \<Rightarrow> doE
+            dest \<leftarrow> without_preemption $ get_cap_reg nbsendRecvDest;
+            handle_invocation False False True dest;
+            without_preemption $ handle_recv True True
+          odE
+        | SysNBSendWait \<Rightarrow> doE
+            reply_cptr \<leftarrow> without_preemption $ get_cap_reg replyRegister;
+            handle_invocation False False True reply_cptr;
+            without_preemption $ handle_recv True False
+          odE
+        | SysWait \<Rightarrow> without_preemption $ handle_recv True False
+        | SysNBWait \<Rightarrow> without_preemption $ handle_recv False False
+        | SysNBRecv \<Rightarrow> without_preemption $ handle_recv False True)
+  odE"
 
 | "handle_event (UnknownSyscall n) = (without_preemption $ do
-    thread \<leftarrow> gets cur_thread;
-    handle_fault thread $ UnknownSyscallException $ of_nat n;
-    return ()
+    update_time_stamp;
+    restart \<leftarrow> check_budget_restart;
+    when restart $ do
+      thread \<leftarrow> gets cur_thread;
+      handle_fault thread $ UnknownSyscallException $ of_nat n
+    od
   od)"
 
 | "handle_event (UserLevelFault w1 w2) = (without_preemption $ do
-    thread \<leftarrow> gets cur_thread;
-    handle_fault thread $ UserException (w1 && mask 32) (w2 && mask 29);
-    return ()
+    update_time_stamp;
+    restart \<leftarrow> check_budget_restart;
+    when restart $ do
+      thread \<leftarrow> gets cur_thread;
+      handle_fault thread $ UserException (w1 && mask 32) (w2 && mask 29)
+    od
   od)"
 
 | "handle_event Interrupt = (without_preemption $ do
@@ -360,9 +403,12 @@ where
   od)"
 
 | "handle_event (VMFaultEvent fault_type) = (without_preemption $ do
-    thread \<leftarrow> gets cur_thread;
-    handle_vm_fault thread fault_type <catch> handle_fault thread;
-    return ()
+    update_time_stamp;
+    restart \<leftarrow> check_budget_restart;
+    when restart $ do
+      thread \<leftarrow> gets cur_thread;
+      handle_vm_fault thread fault_type <catch> handle_fault thread
+    od
   od)"
 
 | "handle_event (HypervisorEvent hypfault_type) = (without_preemption $ do
@@ -380,12 +426,16 @@ text {*
 *}
 
 definition
-  call_kernel :: "event \<Rightarrow> (unit,'z::state_ext_sched) s_monad" where
+  call_kernel :: "event \<Rightarrow> (unit, det_ext) s_monad" where
   "call_kernel ev \<equiv> do
        handle_event ev <handle>
            (\<lambda>_. without_preemption $ do
                   irq \<leftarrow> do_machine_op $ getActiveIRQ True;
-                  when (irq \<noteq> None) $ handle_interrupt (the irq)
+                  when (irq \<noteq> None) $ do
+                    commit \<leftarrow> check_budget;
+                    when commit commit_time;
+                    handle_interrupt (the irq)
+                  od
                 od);
        schedule;
        activate_thread
